ECDSA Exp QED

code/ecdsa/Hacl.Impl.ECDSA.MM.Exponent.fst
@@ -42,66 +42,13 @@ let fromDomainImpl #c a result =
   pop_frame()
 
 
-val lemma_fromDomain1: #c: curve -> a: nat -> 
-  Lemma ((fromDomain_ #c #DSA (fromDomain_ #c #DSA (fromDomain_ #c #DSA a))) == ((a * modp_inv2_prime (pow2 256) prime_p256_order * modp_inv2_prime (pow2 256) prime_p256_order * modp_inv2_prime (pow2 256) prime_p256_order) % prime_p256_order))
-
-let lemma_fromDomain1 a = 
-  let f = modp_inv2_prime (pow2 256) prime_p256_order in 
-  lemma_mod_mul_distr_l (a * f) f prime_p256_order; 
-  lemma_mod_mul_distr_l (a * f * f) f prime_p256_order
-
-
-val lemma_fromDomain2: #c: curve -> a: nat -> 
-  Lemma (pow (fromDomain_ #c #DSA (fromDomain_ #c #DSA a)) (prime_p256_order - 2) % prime_p256_order == 
-    (
-      pow a (prime_p256_order - 2) * 
-      pow (modp_inv2_prime (pow2 256) prime_p256_order) (prime_p256_order - 2) * 
-      pow (modp_inv2_prime (pow2 256) prime_p256_order) (prime_p256_order - 2)) % prime_p256_order /\
-      pow (modp_inv2_prime (pow2 256) prime_p256_order) (prime_p256_order - 2) * pow (pow2 256) (prime_p256_order -2) % prime_p256_order == 1
-    )
-
-
-let lemma_fromDomain2 a = 
-  let r = modp_inv2_prime (pow2 256) prime_p256_order in 
-  lemma_mod_mul_distr_l (a * r) r prime_p256_order;
-  power_distributivity (a * r * r) (prime_p256_order - 2) prime_p256_order;
-    assert_by_tactic (a * r * r == a * (r * r)) canon;
-  power_distributivity_2 a (r * r) (prime_p256_order - 2);
-  power_distributivity_2 (modp_inv2_prime (pow2 256) prime_p256_order) (modp_inv2_prime (pow2 256) prime_p256_order) (prime_p256_order -2);
-  assert_by_tactic (pow a (prime_p256_order - 2) * (
-      pow (modp_inv2_prime (pow2 256) prime_p256_order) (prime_p256_order - 2) * 
-      pow (modp_inv2_prime (pow2 256) prime_p256_order) (prime_p256_order - 2)) == 
-      pow a (prime_p256_order - 2) * 
-      pow (modp_inv2_prime (pow2 256) prime_p256_order) (prime_p256_order - 2) * 
-      pow (modp_inv2_prime (pow2 256) prime_p256_order) (prime_p256_order - 2)) canon;
-
-  let inv_pow256_order = 43790243014242295660885426880012836369732278457577312309071968676491870960761 in 
-  assert_norm (modp_inv2_prime (pow2 256) prime_p256_order == inv_pow256_order);
-  assert_norm (inv_pow256_order * (pow2 256) % prime_p256_order == 1);
-  power_distributivity_2 (inv_pow256_order) (pow2 256) (prime_p256_order - 2);
-  power_distributivity (inv_pow256_order * pow2 256) (prime_p256_order - 2) prime_p256_order;
-  power_one (prime_p256_order -2)
-
-
-let multPower #c a b result = 
-  push_frame();
-    let len = getCoordinateLenU64 c in 
-    let tempB1 = create len (u64 0) in 
-    let buffFromDB = create len (u64 0) in 
-	let h0 = ST.get() in 
-      fromDomainImpl #c a tempB1;
-      fromDomainImpl #c b buffFromDB;
-	let h1 = ST.get() in 
-      fromDomainImpl #c buffFromDB buffFromDB;
-	let h2 = ST.get() in 
-      montgomery_ladder_exponent #c tempB1 tempB1;
-      montgomery_multiplication_buffer_dsa tempB1 buffFromDB result;
-      	let h3 = ST.get() in 
-    pop_frame();
- 
-  let a = as_nat c h0 a in 
-  let b = as_nat c h0 b in 
+val lemma_multPower: #c: curve -> a: nat -> b: nat -> Lemma (
   let order = getOrder #c in 
+  toDomain_ #c #DSA (exponent_spec #c (fromDomain_ #c #DSA (fromDomain_ #c #DSA a)) * fromDomain_ #c #DSA (fromDomain_ #c #DSA (fromDomain_ #c #DSA b)) % order) == 
+  (pow a (order - 2) * b) % order)
+
+let lemma_multPower #c a b = 
+let order = getOrder #c in 
   let r = modp_inv2_prime (pow2 (getPower c)) order in  
 
   lemma_exp_not_zero order (pow2 (getPower c) % order) (order - 2);
@@ -163,36 +110,32 @@ let multPower #c a b result =
 
 
 
+let multPower #c a b result = 
+  push_frame();
+  let len = getCoordinateLenU64 c in 
+  let tempB1 = create len (u64 0) in 
+  let buffFromDB = create len (u64 0) in 
+    let h0 = ST.get() in 
+  fromDomainImpl #c a tempB1;
+  fromDomainImpl #c b buffFromDB;
+    let h1 = ST.get() in 
+  fromDomainImpl #c buffFromDB buffFromDB;
+    let h2 = ST.get() in 
+  montgomery_ladder_exponent #c tempB1 tempB1;
+  montgomery_multiplication_buffer_dsa tempB1 buffFromDB result;
+    let h3 = ST.get() in 
+    pop_frame();
+
+  lemma_multPower #c (as_nat c h0 a) (as_nat c h0 b)
+
+
 let multPowerPartial #c s a b result = 
   let h0 = ST.get() in 
   push_frame();
-    let buffFromDB = create (size 4) (u64 0) in 
+    let len = getCoordinateLenU64 c in 
+    let buffFromDB = create len (u64 0) in 
     fromDomainImpl #c b buffFromDB;
     fromDomainImpl #c buffFromDB buffFromDB;
     montgomery_multiplication_buffer_dsa a buffFromDB result;
   pop_frame();
-
-    let p = pow (fromDomain_ #c #DSA (fromDomain_ #c #DSA (as_nat c h0 s))) (prime_p256_order - 2) % prime_p256_order in 
-    let q = fromDomain_ #c #DSA (fromDomain_ #c #DSA (fromDomain_ #c #DSA (as_nat c h0 b))) in 
-    let r = modp_inv2_prime (pow2 256) prime_p256_order in 
-      lemma_fromDomain1 #c (as_nat c h0 b);
-      lemma_fromDomain2 #c (as_nat c h0 s);
-
-      lemma_mod_mul_distr_l (pow (as_nat c h0 s) (prime_p256_order - 2) * pow r (prime_p256_order - 2) * pow r (prime_p256_order - 2)) (((as_nat c h0 b) * r * r * r) % prime_p256_order) prime_p256_order;
-      lemma_mod_mul_distr_r (pow (as_nat c h0 s) (prime_p256_order - 2) * pow r (prime_p256_order - 2) * pow r (prime_p256_order - 2)) ((as_nat c h0 b) * r * r * r) prime_p256_order;
-      assert_by_tactic (pow (as_nat c h0 s) (prime_p256_order - 2) * pow r (prime_p256_order - 2) * pow r (prime_p256_order - 2) * ((as_nat c h0 b) * r * r * r) == pow (as_nat c h0 s) (prime_p256_order - 2) * (pow r (prime_p256_order - 2) * r) * (pow r (prime_p256_order - 2) * r) * (as_nat c h0 b) * r) canon;
-    
-      pow_plus r (prime_p256_order - 2) 1; 
-      power_one r;
-      lemma_mod_mul_distr_l (pow (as_nat c h0 s) (prime_p256_order - 2) * (pow r (prime_p256_order - 1)) * (pow r (prime_p256_order - 1)) * (as_nat c h0 b) * r) (pow2 256) prime_p256_order;
-      
-      assert_by_tactic (pow (as_nat c h0 s) (prime_p256_order - 2) * (pow r (prime_p256_order - 1)) * (pow r (prime_p256_order - 1)) * (as_nat c h0 b) * r * pow2 256 == pow (as_nat c h0 s) (prime_p256_order - 2) * (pow r (prime_p256_order - 1)) * (pow r (prime_p256_order - 1)) * (as_nat c h0 b) * (r * pow2 256)) canon;
-      lemma_mod_mul_distr_r (pow (as_nat c h0 s) (prime_p256_order - 2) * (pow r (prime_p256_order - 1)) * (pow r (prime_p256_order - 1)) * (as_nat c h0 b)) (r * pow2 256) prime_p256_order;
-      assert_norm ((pow2 256 * modp_inv2_prime (pow2 256) prime_p256_order) % prime_p256_order == 1);
-      
-      assert_by_tactic (pow (as_nat c h0 s) (prime_p256_order - 2) * (pow r (prime_p256_order - 1)) * (pow r (prime_p256_order - 1)) * (as_nat c h0 b) == pow (as_nat c h0 s) (prime_p256_order - 2) * (as_nat c h0 b)  * (pow r (prime_p256_order - 1)) * (pow r (prime_p256_order - 1))) canon;
-      lemma_mod_mul_distr_r (pow (as_nat c h0 s) (prime_p256_order - 2) * (as_nat c h0 b)  * (pow r (prime_p256_order - 1))) (pow r (prime_p256_order - 1)) prime_p256_order;
-      lemma_l_ferm ();
-      
-      lemma_mod_mul_distr_r (pow (as_nat c h0 s) (prime_p256_order - 2) * (as_nat c h0 b)) (pow r (prime_p256_order - 1)) prime_p256_order
-
+  lemma_multPower #c (as_nat c h0 s) (as_nat c h0 b)
